Equivalence.v
@@ -1,0 +1,312 @@
+Require Import Termination.
+Require Import Setoid.
+
+Open Scope t_scope.
+Open Scope list_scope.
+
+Reserved Notation " M ≃ N " (at level 70).
+Inductive Eq2 M N : Prop :=
+| equivT : forall
+    (HTM : nil ⊢ M ::: 2)
+    (HTN : nil ⊢ N ::: 2)
+    (HRedM : M ↦* TT)
+    (HRedN : N ↦* TT),
+    M ≃ N
+| equivF : forall
+    (HTM : nil ⊢ M ::: 2)
+    (HTN : nil ⊢ N ::: 2)
+    (HRedM : M ↦* FF)
+    (HRedN : N ↦* FF),
+    M ≃ N
+where " M ≃ N " := (Eq2 M N).
+
+Lemma step_det : forall M N₁ N₂
+  (Hred₁ : M ↦ N₁)
+  (Hred₂ : M ↦ N₂),
+  N₁ = N₂.
+Proof.
+  intros; generalize dependent N₂; induction Hred₁; intros;
+    try (inversion Hred₂; subst; [reflexivity | inversion HR]);
+      inversion Hred₂; subst; (inversion Hred₁; fail) || f_equal; intuition.
+Qed.
+
+Lemma value_not_red : forall V M
+  (Hval : value V)
+  (Hred : V ↦* M),
+  M = V.
+Proof.
+  induction 2; [reflexivity |].
+  inversion H; subst; inversion Hval.
+Qed.
+  
+Lemma steps_val_det : forall M V₁ V₂
+  (Hval₁ : value V₁)
+  (Hval₂ : value V₂)
+  (Hred₁ : M ↦* V₁)
+  (Hred₂ : M ↦* V₂),
+  V₁ = V₂.
+Proof.
+  intros; generalize dependent V₂; induction Hred₁; intros.
+    symmetry; apply value_not_red; assumption.
+  inversion Hred₂; subst.
+    inversion H; subst; inversion Hval₂.
+  assert (y = y0) by (eauto using step_det); subst.
+  apply IHHred₁; assumption.
+Qed.
+
+Instance Eq2_sym : Symmetric Eq2.
+Proof.
+  intros x.
+  unfold Symmetric; intros.
+  inversion H; auto using Eq2.
+Qed.
+
+Instance Eq2_trans : Transitive Eq2.
+Proof.
+  unfold Transitive; intros.
+  inversion H0; subst; inversion H; subst; auto using Eq2;
+    assert (TT = FF) by (eauto using steps_val_det, value); discriminate.
+Qed.
+
+Lemma Eq2_type_refl : forall M (HT : nil ⊢ M ::: 2), M ≃ M.
+Proof.
+  intros; assert (HR := types_red _ _ _ nil HT I I).
+  simpl in *; inversion HR; subst; auto using Eq2.
+Qed.
+
+Inductive Eqω : te -> te -> Prop :=
+| Eqωz : forall M N (HMz : M ↦* z) (HNz : N ↦* z), Eqω M N
+| Eqωs : forall M N M' N' (HMs : M ↦* s M') (HNs : N ↦* s N') (HEq : Eqω M' N'), Eqω M N.
+
+Instance Eqω_sym : Symmetric Eqω.
+Proof.
+  unfold Symmetric; intros; induction H; eauto using Eqω.
+Qed.    
+
+Instance Eqω_trans : Transitive Eqω.
+Proof.
+  unfold Transitive; intros.
+  revert z H0; induction H; intros u Hu; inversion Hu; subst; eauto using Eqω.
+  assert (z = s M') by (eauto using steps_val_det, value); discriminate.
+  assert (z = s N') by (eauto using steps_val_det, value); discriminate.
+  assert (HT : s N' = s M'0) by (eauto using steps_val_det, value); inversion HT; subst;
+    eauto using Eqω.
+Qed.
+
+CoInductive Eqs (P : te -> te -> Prop) : te -> te -> Prop :=
+| EqS : forall M N (HEqHD : P (hd M) (hd N)) (HEqTL : Eqs P (tl M) (tl N)), Eqs P M N.
+
+Instance Eqs_sym P (HSym : Symmetric P) : Symmetric (Eqs P).
+Proof.
+  unfold Symmetric; cofix; intros x y H.
+  inversion H; subst; constructor.
+    symmetry; assumption.
+  apply Eqs_sym; assumption.
+Qed.
+
+Instance Eqs_trans P (HTran : Transitive P) : Transitive (Eqs P).
+Proof.
+  cofix; unfold Transitive; intros u v w Huv Hvw.
+  inversion Huv; subst; inversion Hvw; subst; constructor.
+    eapply HTran; eassumption.
+  eapply Eqs_trans; eassumption.
+Qed.
+
+Inductive ctx : Type :=
+| hole   : ctx
+| full   : te -> ctx
+| ct_lam : ty -> ctx -> ctx
+| ct_appL: te -> ctx -> ctx
+| ct_appR: te -> ctx -> ctx
+| ct_s   : ctx -> ctx
+| ct_rec0: te -> te -> ctx -> ctx
+| ct_rec1: te -> te -> ctx -> ctx
+| ct_rec2: te -> te -> ctx -> ctx
+| ct_hd  : ctx -> ctx
+| ct_tl  : ctx -> ctx
+| ct_sd0 : te -> te -> ctx -> ctx
+| ct_sd1 : te -> te -> ctx -> ctx
+| ct_sd2 : te -> te -> ctx -> ctx.
+
+Fixpoint plug (E : ctx) (M : te) : te :=
+  match E with
+    | hole           => M
+    | full N         => N
+    | ct_lam A E     => λ A, plug E M
+    | ct_appL N E    => N @ (plug E M)
+    | ct_appR N E    => (plug E M) @ N
+    | ct_s E         => s (plug E M)
+    | ct_rec0 M₀ M₁ E => rec (plug E M) M₀ M₁
+    | ct_rec1 M₀ M₁ E => rec M₀ (plug E M) M₁
+    | ct_rec2 M₀ M₁ E => rec M₀ M₁ (plug E M)
+    | ct_hd E        => hd (plug E M)
+    | ct_tl E        => tl (plug E M)
+    | ct_sd0 M₀ M₁ E  => seed (plug E M) M₀ M₁
+    | ct_sd1 M₀ M₁ E  => seed M₀ (plug E M) M₁
+    | ct_sd2 M₀ M₁ E  => seed M₀ M₁ (plug E M)
+  end.
+
+Reserved Notation " E · F " (at level 40).
+
+Fixpoint compose (E E' : ctx) : ctx :=
+  match E with
+    | hole => E'
+    | full M => E
+    | ct_lam A E => ct_lam A (E · E')
+    | ct_appL M E => ct_appL M (E · E')
+    | ct_appR N E => ct_appR N (E · E')
+    | ct_s E => ct_s (E · E')
+    | ct_rec0 M N E => ct_rec0 M N (E · E')
+    | ct_rec1 M N E => ct_rec1 M N (E · E')
+    | ct_rec2 M N E => ct_rec2 M N (E · E')
+    | ct_hd E => ct_hd (E · E')
+    | ct_tl E => ct_tl (E · E')
+    | ct_sd0 M N E => ct_sd0 M N (E · E')
+    | ct_sd1 M N E => ct_sd1 M N (E · E')
+    | ct_sd2 M N E => ct_sd2 M N (E · E')
+  end where " E · E' " := (compose E E').
+
+Lemma plug_compose : forall M E E',
+  plug E (plug E' M) = plug (E · E') M.
+Proof.
+  induction E; intros; simpl; try rewrite IHE; reflexivity.
+Qed.  
+
+Definition type_context E Γ Δ A B :=
+  forall M (HT : Γ ⊢ M ::: A), Δ ⊢ plug E M ::: B.
+Notation " E ::: [ Γ , A ] → [ Δ , B ] " := (type_context E Γ Δ A B) (at level 70).
+
+Definition obs_eq Γ A (M N : {K : te | Γ ⊢ K ::: A}) :=
+  forall E (HTE : E ::: [ Γ, A ] → [ nil, 2 ]),
+    plug E (proj1_sig M) ≃ plug E (proj1_sig N).
+Notation " Γ ⊢ M == N ::: A " := (obs_eq Γ A M N) (at level 70).
+
+Definition consistent (P : forall Γ A, relation {K : te | Γ ⊢ K ::: A}) :=
+  forall M N, P nil 2 M N -> proj1_sig M ≃ proj1_sig N.
+
+Definition closed (P : forall Γ A, relation {K : te | Γ ⊢ K ::: A}) :=
+  forall E Γ Δ A B M N
+    (HTE  : E ::: [Γ, A] → [Δ, B])
+    (HPMN : P Γ A M N),
+    (P Δ B (exist _ (plug E (proj1_sig M)) (HTE _ (proj2_sig M)))
+      (exist _ (plug E (proj1_sig N)) (HTE _ (proj2_sig N)))).
+
+Record ConsCong (P : forall Γ A, relation {K : te | Γ ⊢ K ::: A}) :=
+  { Cong_Equiv  : forall Γ A, Equivalence (P Γ A);
+    Cong_Cons   : consistent P;
+    Cong_Closed : closed P}.
+
+Lemma obs_eq_cong : ConsCong obs_eq.
+Proof.
+  split; intros.
+  split; unfold Reflexive, Symmetric, Transitive; intros.
+  (* refl *)
+  unfold obs_eq; intros.
+  apply Eq2_type_refl, HTE, (proj2_sig x).
+  (* symm *)
+  unfold obs_eq; intros; symmetry; apply H; assumption.
+  (* tran *)
+  unfold obs_eq; intros; etransitivity; eauto; fail.
+  (* cons *)
+  unfold consistent; intros.
+  specialize (H hole); simpl in H; apply H.
+  intros K HT; simpl; assumption.
+  (* cong *)
+  unfold closed, obs_eq; intros.
+  simpl; rewrite !plug_compose; apply HPMN.
+  intros K HT; rewrite <- plug_compose.
+  apply HTE0, HTE; assumption.
+Qed.
+
+Lemma obs_eq_coarsest :
+  forall (P : forall Γ A, relation {K : te | Γ ⊢ K ::: A})
+    (HCC : ConsCong P)
+    Γ A M N (HIn : P Γ A M N),
+    Γ ⊢ M == N ::: A.
+Proof.
+  unfold obs_eq; intros.
+  assert (HCons := Cong_Cons _ HCC (exist _ (plug E (proj1_sig M)) (HTE _ (proj2_sig M)))
+    (exist _ (plug E (proj1_sig N)) (HTE _ (proj2_sig N)))); simpl in HCons.
+  apply HCons; clear HCons.
+  apply (Cong_Closed _ HCC); assumption.
+Qed.
+
+(* Logical Equivalence *)
+
+Reserved Notation " M ≡ N ::: A " (at level 70).
+
+Fixpoint log_equiv (A : ty) (M N : te) : Prop :=
+  match A with
+    | 2 => M ≃ N
+    | ω => Eqω M N
+    | A₁ → A₂ => forall M' N' (HEq : M' ≡ N' ::: A₁), M ≡ N ::: A₂
+    | stream A => Eqs (log_equiv A) M N
+  end where " M ≡ N ::: A " := (log_equiv A M N) : t_scope.
+
+Instance log_equiv_symm A : Symmetric (log_equiv A).
+Proof.
+  induction A; eauto with typeclass_instances.
+  (* arrow *)
+  unfold Symmetric; simpl; intros.
+  symmetry; eapply H; eassumption.
+  (* stream *)
+  unfold Symmetric; simpl; apply Eqs_sym; assumption.
+Qed.
+
+Instance log_equiv_trans A : Transitive (log_equiv A).
+Proof.
+  induction A; eauto with typeclass_instances.
+  (* arrow *)
+  unfold Transitive; simpl; intros.
+  etransitivity; eauto.
+  (* stream *)
+  unfold Transitive; simpl; apply Eqs_trans; assumption.
+Qed.
+
+Reserved Notation " γ₁ ∼ γ₂ ::: Γ " (at level 70).
+Fixpoint ctx_log_equiv Γ γ₁ γ₂ :=
+  match Γ, γ₁, γ₂ with
+    | nil, nil, nil => True
+    | A :: Γ, M :: γ₁, N :: γ₂ => (M ≡ N ::: A) /\ (γ₁ ∼ γ₂ ::: Γ)
+    | _, _, _ => False
+  end where " γ₁ ∼ γ₂ ::: Γ " := (ctx_log_equiv Γ γ₁ γ₂) : t_scope.
+
+Instance ctx_log_equiv_sym Γ : Symmetric (ctx_log_equiv Γ).
+Proof.
+  induction Γ; unfold Symmetric; intros; destruct x; destruct y;
+    try contradiction; [tauto |].
+  simpl in *; destruct H; split; symmetry; assumption.
+Qed.
+
+Instance ctx_log_equiv_trans Γ : Transitive (ctx_log_equiv Γ).
+Proof.
+  induction Γ; unfold Transitive; intros;
+    destruct x; destruct y; destruct z; try contradiction; [tauto |].
+  simpl in *; destruct H; destruct H0; split; etransitivity; eassumption.
+Qed.
+
+Definition open_simeq Γ A (M N : {K : te | Γ ⊢ K ::: A}) := forall γ₁ γ₂
+  (HEΓ : γ₁ ∼ γ₂ ::: Γ),
+  [γ₁ ! 0](proj1_sig M) ≡ [γ₂ ! 0](proj1_sig N) ::: A.
+Notation " Γ ⊢ M ∼ N ::: A " := (open_simeq Γ A M N) (at level 70) : t_scope.
+
+Instance open_simeq_symm  Γ A : Symmetric (open_simeq Γ A).
+Proof.
+  unfold Symmetric, open_simeq; intros.
+  symmetry; apply H; try symmetry; assumption.
+Qed.  
+
+Lemma open_simeq_trans : forall Γ A, transitive _ (open_simeq Γ A).
+Proof.
+  unfold transitive, open_simeq; intros.
+  etransitivity; [apply H | apply H0]; try eassumption.
+  etransitivity; [symmetry |]; eassumption.
+Qed.
+
+Lemma open_simeq_cons : consistent open_simeq.
+Proof.
+  unfold consistent; intros.
+  apply (H nil nil I).
+Qed.
+
+Scheme types_Ind := Induction for types Sort Prop.
